Runtime/Utilities/Mathlib.lean
@@ -1,8 +1,0 @@
-import Runtime.Utilities.Std
-
-open Lean Meta Elab Term Command in
-elab (name := runCmd) "run_cmd " elems:doSeq : command => do
-  ← liftTermElabM <|
-    unsafe evalTerm (CommandElabM Unit)
-      (mkApp (mkConst ``CommandElabM) (mkConst ``Unit))
-      (← `(discard do $elems))
