lakefile.lean
@@ -3,4 +3,5 @@ open Lake DSL
 
 package reactor_lean
 
+@[default_target]
 lean_lib Runtime
